src/ADTNotation/BuildADT.v
@@ -22,29 +22,352 @@ Class RepHint := {repHint : Type}.
 (* This class is used to give a hint to help infer the
    return type. *)
 
-Class CoDHint := {codHint : Type}.
+Class CoDHint := {codHint : option Type}.
 
 (* Notations for ADT methods. Constructors and methods
    are parameterized by a signature that includes the
    domain (both) and codomain (just methods). *)
 
-Record methDef {Rep : Type} (Sig : methSig) :=
-  { methBody :> methodType Rep (methDom Sig) (methCod Sig)}.
-
-Notation "'Def' 'Method' id ( r : 'rep' ) x1 .. xn : cod := bod" :=
-  (Build_methDef {| methID := id; methDom := _; methCod := cod |} (fun r => (fun x1 => .. (fun xn =>  bod%comp) ..)))
-    (no associativity, id at level 0, r at level 0, x1 closed binder,
-     xn closed binder, cod at level 0,
-     at level 94, format "'Def'  'Method'  id  (  r  :  'rep'  )  x1  ..  xn  :  cod  :=  '/' '[  '   bod ']' " ) :
-methDef_scope.
-
-Delimit Scope methDefParsing_scope with methDefParsing.
-Delimit Scope methDef_scope with methDef.
-
 Record consDef {Rep : Type} (Sig : consSig) :=
   { consBody :> constructorType Rep (consDom Sig) }.
 
 Delimit Scope consDef_scope with consDef.
+
+(* Notations for parsing Constructors. Including the arity is the simplest way to
+ make typechecking work. *)
+Notation "'Def' 'Constructor0' id : 'rep' := bod" :=
+  (Build_consDef _ {| consID := id; consDom := [] |} ((bod%comp : constructorType repHint [ ]) ))
+    (no associativity, at level 94, id at level 0,
+     x1 closed binder, xn closed binder,
+     format "'Def'  'Constructor0'  id  :  'rep'  :=  '/' '[  '   bod ']' " ) :
+    consDef_scope.
+
+Notation "'Def' 'Constructor1' id x1 .. xn : 'rep' := bod" :=
+  (Build_consDef _ {| consID := id; consDom := [_] |} ((fun x1 => .. ((fun xn => (bod%comp : constructorType repHint [ ]) )) ..)))
+    (no associativity, at level 94, id at level 0,
+     x1 closed binder, xn closed binder,
+     format "'Def'  'Constructor1'  id  x1  ..  xn  :  'rep'  :=  '/' '[  '   bod ']' " ) :
+    consDef_scope.
+
+Notation "'Def' 'Constructor2' id x1 .. xn : 'rep' := bod" :=
+  (Build_consDef _ {| consID := id; consDom := [_; _] |} ((fun x1 => .. ((fun xn => (bod%comp : constructorType repHint [ ]) )) ..)))
+    (no associativity, at level 94, id at level 0,
+     x1 closed binder, xn closed binder,
+     format "'Def'  'Constructor2'  id  x1  ..  xn  :  'rep'  :=  '/' '[  '   bod ']' " ) :
+    consDef_scope.
+
+Notation "'Def' 'Constructor3' id x1 .. xn : 'rep' := bod" :=
+  (Build_consDef _ {| consID := id; consDom := [_; _; _] |} ((fun x1 => .. ((fun xn => (bod%comp : constructorType repHint [ ]) )) ..)))
+    (no associativity, at level 94, id at level 0,
+     x1 closed binder, xn closed binder,
+     format "'Def'  'Constructor3'  id  x1  ..  xn  :  'rep'  :=  '/' '[  '   bod ']' " ) :
+    consDef_scope.
+
+Notation "'Def' 'Constructor4' id x1 .. xn : 'rep' := bod" :=
+  (Build_consDef _ {| consID := id; consDom := [_; _; _ ; _] |} ((fun x1 => .. ((fun xn => (bod%comp : constructorType repHint [ ]) )) ..)))
+    (no associativity, at level 94, id at level 0,
+     x1 closed binder, xn closed binder,
+     format "'Def'  'Constructor4'  id  x1  ..  xn  :  'rep'  :=  '/' '[  '   bod ']' " ) :
+    consDef_scope.
+
+Notation "'Def' 'Constructor5' id x1 .. xn : 'rep' := bod" :=
+  (Build_consDef _ {| consID := id; consDom := [_; _; _; _; _] |} ((fun x1 => .. ((fun xn => (bod%comp : constructorType repHint [ ]) )) ..)))
+    (no associativity, at level 94, id at level 0,
+     x1 closed binder, xn closed binder,
+     format "'Def'  'Constructor5'  id  x1  ..  xn  :  'rep'  :=  '/' '[  '   bod ']' " ) :
+    consDef_scope.
+
+Notation "'Def' 'Constructor6' id x1 .. xn : 'rep' := bod" :=
+  (Build_consDef _ {| consID := id; consDom := [_; _; _; _;_; _] |} ((fun x1 => .. ((fun xn => (bod%comp : constructorType repHint [ ]) )) ..)))
+    (no associativity, at level 94, id at level 0,
+     x1 closed binder, xn closed binder,
+     format "'Def'  'Constructor6'  id  x1  ..  xn  :  'rep'  :=  '/' '[  '   bod ']' " ) :
+    consDef_scope.
+
+Notation "'Def' 'Constructor7' id x1 .. xn : 'rep' := bod" :=
+  (Build_consDef _ {| consID := id; consDom := [_; _; _; _; _; _; _] |} ((fun x1 => .. ((fun xn => (bod%comp : constructorType repHint [ ]) )) ..)))
+    (no associativity, at level 94, id at level 0,
+     x1 closed binder, xn closed binder,
+     format "'Def'  'Constructor7'  id  x1  ..  xn  :  'rep'  :=  '/' '[  '   bod ']' " ) :
+    consDef_scope.
+
+Notation "'Def' 'Constructor8' id x1 .. xn : 'rep' := bod" :=
+  (Build_consDef _ {| consID := id; consDom := [_; _; _; _; _; _; _ ; _] |} ((fun x1 => .. ((fun xn => (bod%comp : constructorType repHint [ ]) )) ..)))
+    (no associativity, at level 94, id at level 0,
+     x1 closed binder, xn closed binder,
+     format "'Def'  'Constructor8'  id  x1  ..  xn  :  'rep'  :=  '/' '[  '   bod ']' " ) :
+    consDef_scope.
+
+Notation "'Def' 'Constructor9' id x1 .. xn : 'rep' := bod" :=
+  (Build_consDef _ {| consID := id; consDom := [_; _; _; _; _; _; _; _; _] |} ((fun x1 => .. ((fun xn => (bod%comp : constructorType repHint [ ]) )) ..)))
+    (no associativity, at level 94, id at level 0,
+     x1 closed binder, xn closed binder,
+     format "'Def'  'Constructor9'  id  x1  ..  xn  :  'rep'  :=  '/' '[  '   bod ']' " ) :
+    consDef_scope.
+
+Notation "'Def' 'Constructor10' id x1 .. xn : 'rep' := bod" :=
+  (Build_consDef _ {| consID := id; consDom := [_; _; _; _; _; _; _; _;  _; _] |} ((fun x1 => .. ((fun xn => (bod%comp : constructorType repHint [ ]) )) ..)))
+    (no associativity, at level 94, id at level 0,
+     x1 closed binder, xn closed binder,
+     format "'Def'  'Constructor10'  id  x1  ..  xn  :  'rep'  :=  '/' '[  '   bod ']' " ) :
+    consDef_scope.
+
+(* Once the type infomation is in hand, two rules can handle pretty printing.  *)
+Notation "'Def' 'Constructor' id x1 .. xn : 'rep' := bod" :=
+  (Build_consDef _ {| consID := id; consDom := _ |} ((fun x1 => .. ((fun xn => bod%comp )) ..)))
+    (no associativity, at level 94, id at level 0,
+     x1 closed binder, xn closed binder,
+     format "'Def'  'Constructor'  id  x1  ..  xn  :  'rep'  :=  '/' '[  '   bod ']' " ) :
+    consDef_scope.
+
+Notation "'Def' 'Constructor' id : 'rep' := bod" :=
+  (Build_consDef _ {| consID := id; consDom := [] |} bod%comp)
+    (no associativity, at level 94, id at level 0,
+     format "'Def'  'Constructor'  id :  'rep'  :=  '/' '[  '   bod ']' " ) :
+    consDef_scope.
+
+(* Notations for parsing methods. Again, including the arity is the simplest way to
+ make typechecking work. *)
+
+Record methDef {Rep : Type} (Sig : methSig) :=
+  { methBody :> methodType Rep (methDom Sig) (methCod Sig)}.
+
+Notation "'Def' 'Method0' id ( r : 'rep' ) : 'rep' '*' cod := bod" :=
+  (Build_methDef {| methID := id; methDom := [] ; methCod := Some (cod : Type) |} (fun r =>
+                                                                                     (let _ := {| codHint := Some (cod : Type) |} in (bod%comp : methodType' _ [] codHint ))))
+    (no associativity, id at level 0, r at level 0, x1 closed binder , xn closed binder, dom at level 0,
+     cod at level 0, only parsing,
+     at level 94,
+     format "'Def'  'Method0'  id  (  r  :  'rep'  )  :  'rep'  '*'  cod  :=  '/' '[  '   bod ']' ")
+  : methDefParsing_scope.
+
+Notation "'Def' 'Method1' id ( r : 'rep' ) x1 .. xn : 'rep' '*' cod := bod" :=
+  (Build_methDef {| methID := id; methDom := [_] ; methCod := Some (cod : Type) |} (fun r =>
+                                                                                      (fun x1 => .. (fun xn => let _ := {| codHint := Some (cod : Type) |} in (bod%comp : methodType' _ [] codHint )) ..)))
+    (no associativity, id at level 0, r at level 0, x1 closed binder , xn closed binder, dom at level 0,
+     only parsing,
+     at level 94,
+     format "'Def'  'Method1'  id  (  r  :  'rep'  )  x1  ..  xn  :  'rep'  '*'  cod  :=  '/' '[  '   bod ']' ")
+  : methDefParsing_scope.
+
+Notation "'Def' 'Method2' id ( r : 'rep' ) x1 .. xn : 'rep' '*' cod := bod" :=
+  (Build_methDef {| methID := id; methDom := [_; _] ; methCod := Some (cod : Type) |} (fun r =>
+                                                                                         (fun x1 => .. (fun xn => let _ := {| codHint := Some (cod : Type) |} in (bod%comp : methodType' _ [] codHint )) ..)))
+    (no associativity, id at level 0, r at level 0, x1 closed binder , xn closed binder, dom at level 0,
+     cod at level 0, only parsing,
+     at level 94,
+     format "'Def'  'Method2'  id  (  r  :  'rep'  )  x1  ..  xn  :  'rep'  '*'  cod  :=  '/' '[  '   bod ']' ")
+  : methDefParsing_scope.
+
+Notation "'Def' 'Method3' id ( r : 'rep' ) x1 .. xn : 'rep' '*' cod := bod" :=
+  (Build_methDef {| methID := id; methDom := [_; _; _] ; methCod := Some (cod : Type) |} (fun r =>
+                                                                                            (fun x1 => .. (fun xn => let _ := {| codHint := Some (cod : Type) |} in (bod%comp : methodType' _ [] codHint )) ..)))
+    (no associativity, id at level 0, r at level 0, x1 closed binder , xn closed binder, dom at level 0,
+     cod at level 0, only parsing,
+     at level 94,
+     format "'Def'  'Method3'  id  (  r  :  'rep'  )  x1  ..  xn  :  'rep'  '*'  cod  :=  '/' '[  '   bod ']' ")
+  : methDefParsing_scope.
+
+Notation "'Def' 'Method4' id ( r : 'rep' ) x1 .. xn : 'rep' '*' cod := bod" :=
+  (Build_methDef {| methID := id; methDom := [_; _; _; _] ; methCod := Some (cod : Type) |} (fun r =>
+                                                                                               (fun x1 => .. (fun xn => let _ := {| codHint := Some (cod : Type) |} in (bod%comp : methodType' _ [] codHint )) ..)))
+    (no associativity, id at level 0, r at level 0, x1 closed binder , xn closed binder, dom at level 0,
+     cod at level 0, only parsing,
+     at level 94,
+     format "'Def'  'Method4'  id  (  r  :  'rep'  )  x1  ..  xn  :  'rep'  '*'  cod  :=  '/' '[  '   bod ']' ")
+  : methDefParsing_scope.
+
+Notation "'Def' 'Method5' id ( r : 'rep' ) x1 .. xn : 'rep' '*' cod := bod" :=
+  (Build_methDef {| methID := id; methDom := [_; _; _; _; _] ; methCod := Some (cod : Type) |} (fun r =>
+                                                                                                  (fun x1 => .. (fun xn => let _ := {| codHint := Some (cod : Type) |} in (bod%comp : methodType' _ [] codHint )) ..)))
+    (no associativity, id at level 0, r at level 0, x1 closed binder , xn closed binder, dom at level 0,
+     cod at level 0, only parsing,
+     at level 94,
+     format "'Def'  'Method5'  id  (  r  :  'rep'  )  x1  ..  xn  :  'rep'  '*'  cod  :=  '/' '[  '   bod ']' ")
+  : methDefParsing_scope.
+
+Notation "'Def' 'Method6' id ( r : 'rep' ) x1 .. xn : 'rep' '*' cod := bod" :=
+  (Build_methDef {| methID := id; methDom := [_; _; _; _; _; _] ; methCod := Some (cod : Type) |} (fun r =>
+                                                                                                     (fun x1 => .. (fun xn => let _ := {| codHint := Some (cod : Type) |} in (bod%comp : methodType' _ [] codHint )) ..)))
+    (no associativity, id at level 0, r at level 0, x1 closed binder , xn closed binder, dom at level 0,
+     cod at level 0, only parsing,
+     at level 94,
+     format "'Def'  'Method6'  id  (  r  :  'rep'  )  x1  ..  xn  :  'rep'  '*'  cod  :=  '/' '[  '   bod ']' ")
+  : methDefParsing_scope.
+
+Notation "'Def' 'Method7' id ( r : 'rep' ) x1 .. xn : 'rep' '*' cod := bod" :=
+  (Build_methDef {| methID := id; methDom := [_; _; _; _; _; _; _] ; methCod := Some (cod : Type) |} (fun r =>
+                                                                                                        (fun x1 => .. (fun xn => let _ := {| codHint := Some (cod : Type) |} in (bod%comp : methodType' _ [] codHint )) ..)))
+    (no associativity, id at level 0, r at level 0, x1 closed binder , xn closed binder, dom at level 0,
+     cod at level 0, only parsing,
+     at level 94,
+     format "'Def'  'Method7'  id  (  r  :  'rep'  )  x1  ..  xn  :  'rep'  '*'  cod  :=  '/' '[  '   bod ']' ")
+  : methDefParsing_scope.
+
+Notation "'Def' 'Method8' id ( r : 'rep' ) x1 .. xn : 'rep' '*' cod := bod" :=
+  (Build_methDef {| methID := id; methDom := [_; _; _; _; _; _; _; _] ; methCod := Some (cod : Type) |} (fun r =>
+                                                                                                           (fun x1 => .. (fun xn => let _ := {| codHint := Some (cod : Type) |} in (bod%comp : methodType' _ [] codHint )) ..)))
+    (no associativity, id at level 0, r at level 0, x1 closed binder , xn closed binder, dom at level 0,
+     cod at level 0, only parsing,
+     at level 94,
+     format "'Def'  'Method8'  id  (  r  :  'rep'  )  x1  ..  xn  :  'rep'  '*'  cod  :=  '/' '[  '   bod ']' ")
+  : methDefParsing_scope.
+
+Notation "'Def' 'Method9' id ( r : 'rep' ) x1 .. xn : 'rep' '*' cod := bod" :=
+  (Build_methDef {| methID := id; methDom := [_; _; _; _; _; _; _; _; _] ; methCod := Some (cod : Type) |} (fun r =>
+                                                                                                              (fun x1 => .. (fun xn => let _ := {| codHint := Some (cod : Type) |} in (bod%comp : methodType' _ [] codHint )) ..)))
+    (no associativity, id at level 0, r at level 0, x1 closed binder , xn closed binder, dom at level 0,
+     cod at level 0, only parsing,
+     at level 94,
+     format "'Def'  'Method9'  id  (  r  :  'rep'  )  x1  ..  xn  :  'rep'  '*'  cod  :=  '/' '[  '   bod ']' ")
+  : methDefParsing_scope.
+
+Notation "'Def' 'Method10' id ( r : 'rep' ) x1 .. xn : 'rep' '*' cod := bod" :=
+  (Build_methDef {| methID := id; methDom := [_; _; _; _; _; _; _; _; _; _] ; methCod := Some (cod : Type) |} (fun r =>
+                                                                                                                 (fun x1 => .. (fun xn => let _ := {| codHint := Some (cod : Type) |} in (bod%comp : methodType' _ [] codHint )) ..)))
+    (no associativity, id at level 0, r at level 0, x1 closed binder , xn closed binder, dom at level 0,
+     cod at level 0, only parsing,
+     at level 94,
+     format "'Def'  'Method10'  id  (  r  :  'rep'  )  x1  ..  xn  :  'rep'  '*'  cod  :=  '/' '[  '   bod ']' ")
+  : methDefParsing_scope.
+
+Notation "'Def' 'Method0' id ( r : 'rep' ) : 'rep' := bod" :=
+  (Build_methDef {| methID := id; methDom := [] ; methCod := None |} (fun r =>
+                                                                        (let _ := {| codHint := None |} in (bod%comp : methodType' _ [] codHint ))))
+    (no associativity, id at level 0, r at level 0, x1 closed binder , xn closed binder, dom at level 0,
+     cod at level 0, only parsing,
+     at level 94,
+     format "'Def'  'Method0'  id  (  r  :  'rep'  )  :  'rep'  :=  '/' '[  '   bod ']' ")
+  : methDefParsing_scope.
+
+Notation "'Def' 'Method1' id ( r : 'rep' ) x1 .. xn : 'rep' := bod" :=
+  (Build_methDef {| methID := id; methDom := [_] ; methCod := None |} (fun r =>
+                                                                         (fun x1 => .. (fun xn => let _ := {| codHint := None |} in (bod%comp : methodType' _ [] codHint )) ..)))
+    (no associativity, id at level 0, r at level 0, x1 closed binder , xn closed binder, dom at level 0,
+     only parsing,
+     at level 94,
+     format "'Def'  'Method1'  id  (  r  :  'rep'  )  x1  ..  xn  :  'rep'  :=  '/' '[  '   bod ']' ")
+  : methDefParsing_scope.
+
+Notation "'Def' 'Method2' id ( r : 'rep' ) x1 .. xn : 'rep' := bod" :=
+  (Build_methDef {| methID := id; methDom := [_; _] ; methCod := None |} (fun r =>
+                                                                            (fun x1 => .. (fun xn => let _ := {| codHint := None |} in (bod%comp : methodType' _ [] codHint )) ..)))
+    (no associativity, id at level 0, r at level 0, x1 closed binder , xn closed binder, dom at level 0,
+     cod at level 0, only parsing,
+     at level 94,
+     format "'Def'  'Method2'  id  (  r  :  'rep'  )  x1  ..  xn  :  'rep'  :=  '/' '[  '   bod ']' ")
+  : methDefParsing_scope.
+
+Notation "'Def' 'Method3' id ( r : 'rep' ) x1 .. xn : 'rep' := bod" :=
+  (Build_methDef {| methID := id; methDom := [_; _; _] ; methCod := None |} (fun r =>
+                                                                               (fun x1 => .. (fun xn => let _ := {| codHint := None |} in (bod%comp : methodType' _ [] codHint )) ..)))
+    (no associativity, id at level 0, r at level 0, x1 closed binder , xn closed binder, dom at level 0,
+     cod at level 0, only parsing,
+     at level 94,
+     format "'Def'  'Method3'  id  (  r  :  'rep'  )  x1  ..  xn  :  'rep'  :=  '/' '[  '   bod ']' ")
+  : methDefParsing_scope.
+
+Notation "'Def' 'Method4' id ( r : 'rep' ) x1 .. xn : 'rep' := bod" :=
+  (Build_methDef {| methID := id; methDom := [_; _; _; _] ; methCod := None |} (fun r =>
+                                                                                  (fun x1 => .. (fun xn => let _ := {| codHint := None |} in (bod%comp : methodType' _ [] codHint )) ..)))
+    (no associativity, id at level 0, r at level 0, x1 closed binder , xn closed binder, dom at level 0,
+     cod at level 0, only parsing,
+     at level 94,
+     format "'Def'  'Method4'  id  (  r  :  'rep'  )  x1  ..  xn  :  'rep'  :=  '/' '[  '   bod ']' ")
+  : methDefParsing_scope.
+
+Notation "'Def' 'Method5' id ( r : 'rep' ) x1 .. xn : 'rep' := bod" :=
+  (Build_methDef {| methID := id; methDom := [_; _; _; _; _] ; methCod := None |} (fun r =>
+                                                                                     (fun x1 => .. (fun xn => let _ := {| codHint := None |} in (bod%comp : methodType' _ [] codHint )) ..)))
+    (no associativity, id at level 0, r at level 0, x1 closed binder , xn closed binder, dom at level 0,
+     cod at level 0, only parsing,
+     at level 94,
+     format "'Def'  'Method5'  id  (  r  :  'rep'  )  x1  ..  xn  :  'rep'  :=  '/' '[  '   bod ']' ")
+  : methDefParsing_scope.
+
+Notation "'Def' 'Method6' id ( r : 'rep' ) x1 .. xn : 'rep' := bod" :=
+  (Build_methDef {| methID := id; methDom := [_; _; _; _; _; _] ; methCod := None |} (fun r =>
+                                                                                        (fun x1 => .. (fun xn => let _ := {| codHint := None |} in (bod%comp : methodType' _ [] codHint )) ..)))
+    (no associativity, id at level 0, r at level 0, x1 closed binder , xn closed binder, dom at level 0,
+     cod at level 0, only parsing,
+     at level 94,
+     format "'Def'  'Method6'  id  (  r  :  'rep'  )  x1  ..  xn  :  'rep'  :=  '/' '[  '   bod ']' ")
+  : methDefParsing_scope.
+
+Notation "'Def' 'Method7' id ( r : 'rep' ) x1 .. xn : 'rep' := bod" :=
+  (Build_methDef {| methID := id; methDom := [_; _; _; _; _; _; _] ; methCod := None |} (fun r =>
+                                                                                           (fun x1 => .. (fun xn => let _ := {| codHint := None |} in (bod%comp : methodType' _ [] codHint )) ..)))
+    (no associativity, id at level 0, r at level 0, x1 closed binder , xn closed binder, dom at level 0,
+     cod at level 0, only parsing,
+     at level 94,
+     format "'Def'  'Method7'  id  (  r  :  'rep'  )  x1  ..  xn  :  'rep'  :=  '/' '[  '   bod ']' ")
+  : methDefParsing_scope.
+
+Notation "'Def' 'Method8' id ( r : 'rep' ) x1 .. xn : 'rep' := bod" :=
+  (Build_methDef {| methID := id; methDom := [_; _; _; _; _; _; _; _] ; methCod := None |} (fun r =>
+                                                                                              (fun x1 => .. (fun xn => let _ := {| codHint := None |} in (bod%comp : methodType' _ [] codHint )) ..)))
+    (no associativity, id at level 0, r at level 0, x1 closed binder , xn closed binder, dom at level 0,
+     cod at level 0, only parsing,
+     at level 94,
+     format "'Def'  'Method8'  id  (  r  :  'rep'  )  x1  ..  xn  :  'rep'  :=  '/' '[  '   bod ']' ")
+  : methDefParsing_scope.
+
+Notation "'Def' 'Method9' id ( r : 'rep' ) x1 .. xn : 'rep' := bod" :=
+  (Build_methDef {| methID := id; methDom := [_; _; _; _; _; _; _; _; _] ; methCod := None |} (fun r =>
+                                                                                                 (fun x1 => .. (fun xn => let _ := {| codHint := None |} in (bod%comp : methodType' _ [] codHint )) ..)))
+    (no associativity, id at level 0, r at level 0, x1 closed binder , xn closed binder, dom at level 0,
+     cod at level 0, only parsing,
+     at level 94,
+     format "'Def'  'Method9'  id  (  r  :  'rep'  )  x1  ..  xn  :  'rep'  :=  '/' '[  '   bod ']' ")
+  : methDefParsing_scope.
+
+Notation "'Def' 'Method10' id ( r : 'rep' ) x1 .. xn : 'rep' := bod" :=
+  (Build_methDef {| methID := id; methDom := [_; _; _; _; _; _; _; _; _; _] ; methCod := None |} (fun r =>
+                                                                                                    (fun x1 => .. (fun xn => let _ := {| codHint := None |} in (bod%comp : methodType' _ [] codHint )) ..)))
+    (no associativity, id at level 0, r at level 0, x1 closed binder , xn closed binder, dom at level 0,
+     cod at level 0, only parsing,
+     at level 94,
+     format "'Def'  'Method10'  id  (  r  :  'rep'  )  x1  ..  xn  :  'rep'  :=  '/' '[  '   bod ']' ")
+  : methDefParsing_scope.
+
+(* Again, pretty printing involves fewer rules. *)
+Notation "'Def' 'Method' id ( r : 'rep' ) : 'rep' '*' cod := bod" :=
+  (Build_methDef {| methID := id; methDom := [] ; methCod := Some cod |} (fun r => bod%comp ))
+    (no associativity, id at level 0, r at level 0, x1 closed binder , xn closed binder, dom at level 0,
+     cod at level 0, only parsing,
+     at level 94,
+     format "'Def'  'Method'  id  ( r  :  'rep' )  :  'rep'  '*'  cod  :=  '/' '[  '   bod ']' ")
+  : methDef_scope.
+
+Notation "'Def' 'Method' id ( r : 'rep' ) x1 .. xn : 'rep' '*' cod := bod" :=
+  (Build_methDef {| methID := id; methDom := [_] ; methCod := Some cod |} (fun r =>
+                                                                             (fun x1 => .. (fun xn => (bod%comp )) ..)))
+    (no associativity, id at level 0, r at level 0, x1 closed binder , xn closed binder, dom at level 0,
+     only parsing,
+     at level 94,
+     format "'Def'  'Method'  id  ( r  :  'rep' )  x1  ..  xn  :  'rep'  '*'  cod  :=  '/' '[  '   bod ']' ")
+  : methDef_scope.
+
+Notation "'Def' 'Method' id ( r : 'rep' ) : 'rep' := bod" :=
+  (Build_methDef {| methID := id; methDom := [] ; methCod := None |} (fun r => bod%comp ))
+    (no associativity, id at level 0, r at level 0, x1 closed binder , xn closed binder, dom at level 0,
+     cod at level 0, only parsing,
+     at level 94,
+     format "'Def'  'Method'  id  ( r  :  'rep' )  :  'rep'  :=  '/' '[  '   bod ']' ")
+  : methDef_scope.
+
+Notation "'Def' 'Method' id ( r : 'rep' ) x1 .. xn : 'rep' := bod" :=
+  (Build_methDef {| methID := id; methDom := [_] ; methCod := None |} (fun r =>
+                                                                         (fun x1 => .. (fun xn => (bod%comp )) ..)))
+    (no associativity, id at level 0, r at level 0, x1 closed binder , xn closed binder, dom at level 0,
+     only parsing,
+     at level 94,
+     format "'Def'  'Method'  id  ( r  :  'rep' )  x1  ..  xn  :  'rep'  :=  '/' '[  '   bod ']' ")
+  : methDef_scope.
+
+Delimit Scope methDefParsing_scope with methDefParsing.
+Delimit Scope methDef_scope with methDef.
+
 
 (* Lookup functions for constructor and method definitions. Because
    these definitions are parameterized on a signature, their
@@ -57,7 +380,7 @@ Definition getConsDef
            (consSigs : Vector.t consSig n)
            (consDefs : ilist consSigs)
            (idx : Fin.t n)
-: constructorType Rep (consDom (Vector.nth consSigs idx)) :=
+  : constructorType Rep (consDom (Vector.nth consSigs idx)) :=
   consBody (ith consDefs idx).
 
 Definition getMethDef
@@ -66,10 +389,10 @@ Definition getMethDef
            (methSigs : Vector.t methSig n)
            (methDefs : ilist (B := @methDef Rep) methSigs)
            (idx : Fin.t n)
-: methodType
-    Rep
-    (methDom (Vector.nth methSigs idx))
-    (methCod (Vector.nth methSigs idx)) :=
+  : methodType
+      Rep
+      (methDom (Vector.nth methSigs idx))
+      (methCod (Vector.nth methSigs idx)) :=
   methBody (ith methDefs idx).
 
 (* Always simplify method lookup when the index is specified. *)
@@ -85,17 +408,17 @@ Arguments getMethDef [_] {n} [_] _ idx%string / _ .
 Definition DecoratedADT (dSig : DecoratedADTSig) := ADT dSig.
 
 Definition BuildADT
-        {Rep : Type}
-        {n n'}
-        {consSigs : Vector.t consSig n}
-        {methSigs : Vector.t methSig n'}
-        (consDefs : ilist (B := @consDef Rep) consSigs)
-        (methDefs : ilist (B := @methDef Rep) methSigs)
+           {Rep : Type}
+           {n n'}
+           {consSigs : Vector.t consSig n}
+           {methSigs : Vector.t methSig n'}
+           (consDefs : ilist (B := @consDef Rep) consSigs)
+           (methDefs : ilist (B := @methDef Rep) methSigs)
   : DecoratedADT (BuildADTSig consSigs methSigs)
   := @Build_ADT (BuildADTSig consSigs methSigs)
-               Rep
-               (getConsDef consDefs)
-               (getMethDef methDefs).
+                Rep
+                (getConsDef consDefs)
+                (getMethDef methDefs).
 
 (* Notation for ADTs built from [BuildADT]. *)
 
@@ -113,9 +436,11 @@ Definition callADTMethod
            (idx : BoundedIndex (MethodNames dSig))
   := Methods adt (idxMap idx).
 
+Delimit Scope ADTParsing_scope with ADTParsing.
+
 Notation "'ADTRep' r { cons1 , meth1 , .. , methn } " :=
   (let _ := {| repHint := r |} in
-    @BuildADT r
+   @BuildADT r
              _ _
              _ _
              (icons cons1%consDef (@inil _ (@consDef r)))
@@ -134,64 +459,56 @@ Notation "'ADTRep' r { cons1 , meth1 , .. , methn } " :=
 
 (* Notations for method calls. *)
 Notation callMeth adt idx := (callADTMethod adt (fun idx => ibound (indexb idx))
-                                             {| bindex := idx |}).
+                                            {| bindex := idx |}).
 Notation callCons adt idx := (callADTConstructor adt (fun idx => ibound (indexb idx))
-                                                  {| bindex := idx |}).
+                                                 {| bindex := idx |}).
 
-Section CacheADT.
+Section NotationExample.
 
   Variable Key : Type.
   Variable Value : Type.
-
-  Definition CacheSig : ADTSig :=
-    ADTsignature {
-        Constructor "EmptyCache"  : [ unit : Type ] -> rep,
-        Method "AddKey" : rep x [Key] -> rep x bool ,
-        Method "UpdateKey" : rep x [Key; (Value -> Value)] -> rep x bool ,
-        Method "LookupKey" :  rep x [Key ] -> rep x (option Value)
-  }%ADTSig.
 
   Definition EnsembleInsert  {A} (a : A) (ens : Ensemble A) (a' : A)
     : Prop := a' = a \/ ens a'.
 
   Definition SubEnsembleInsert {A} (a : A) (ens ens' : Ensemble A)
-  : Prop :=
+    : Prop :=
     forall (a' : A), ens' a' -> EnsembleInsert a ens a'.
 
   Definition EnsembleRemove
              (k : Key)
              (ens : Ensemble (Key * Value))
              (k' : Key * Value)
-  : Prop := (fst k' <> k /\ ens k').
+    : Prop := (fst k' <> k /\ ens k').
 
   Definition EnsembleReplace
              (k : Key * Value)
              (ens : Ensemble (Key * Value))
              (k' : Key * Value)
-  : Prop := k' = k \/
-            (EnsembleRemove (fst k) ens k').
+    : Prop := k' = k \/
+              (EnsembleRemove (fst k) ens k').
 
   Definition EnsembleUpdate
              (k : Key)
              (ens : Ensemble (Key * Value))
              (f : Value -> Value)
              (kv : Key * Value)
-  : Prop := ((fst kv) = k /\ exists v, (snd kv) = f v /\ Ensembles.In _ ens (k, v)) \/
-            (EnsembleRemove k ens kv).
+    : Prop := ((fst kv) = k /\ exists v, (snd kv) = f v /\ Ensembles.In _ ens (k, v)) \/
+              (EnsembleRemove k ens kv).
 
   Lemma SubEnsembleInsertReplace
-  : forall (kv : Key * Value)
-           (r : Ensemble (Key * Value)),
-   SubEnsembleInsert kv r (EnsembleReplace kv r).
+    : forall (kv : Key * Value)
+             (r : Ensemble (Key * Value)),
+      SubEnsembleInsert kv r (EnsembleReplace kv r).
   Proof.
     unfold SubEnsembleInsert, EnsembleInsert,
     EnsembleReplace, EnsembleRemove; intros; intuition.
   Qed.
 
   Lemma SubEnsembleInsertRefl
-  : forall (kv : Key * Value)
-           (r : Ensemble (Key * Value)),
-   SubEnsembleInsert kv r r.
+    : forall (kv : Key * Value)
+             (r : Ensemble (Key * Value)),
+      SubEnsembleInsert kv r r.
   Proof.
     unfold SubEnsembleInsert, EnsembleInsert,
     EnsembleReplace, EnsembleRemove; intros; eauto.
@@ -201,60 +518,37 @@ Section CacheADT.
              (r : Ensemble (Key * Value))
              (k : Key)
              (v : option Value)
-  : Prop := forall v', v = Some v' -> r (k, v').
+    : Prop := forall v', v = Some v' -> r (k, v').
 
   Definition usedKey
              (r : Ensemble (Key * Value))
              (k : Key)
-  : Prop := exists v, r (k, v).
+    : Prop := exists v, r (k, v).
 
-Notation "'Def' 'Method' id ( r : 'rep' ) x1 .. xn : cod := bod" :=
-  (Build_methDef {| methID := id; methDom := [_; _ ] ; methCod := cod |} (fun r =>
-                                                                     (fun x1 => .. (fun xn => let cod := {| codHint := cod |} in bod%comp) ..)))
-    (no associativity, id at level 0, r at level 0, x1 closed binder , xn closed binder, dom at level 0,
-     cod at level 0, only parsing,
-     at level 94,
-     format "'Def'  'Method'  id  (  r  :  'rep'  )  x1  ..  xn  :  cod  :=  '/' '[  '   bod ']' ")
-  : methDefParsing_scope.
+  Definition CacheSig : ADTSig :=
+    ADTsignature {
+        Constructor "EmptyCache" : rep,
+        Method "AddKey" : rep * Key * Value -> rep * bool ,
+        Method "UpdateKey" : rep * Key * (Value -> Value) -> rep * bool ,
+        Method "LookupKey" :  rep * Key -> rep * (option Value)
+      }%ADTSig.
 
-Notation "'Def' 'Constructor' id x1 .. xn : 'rep' := bod" :=
-  (Build_consDef _ {| consID := id; consDom := (cons tt ( .. (cons tt nil) ..)) |} (fun x1 => .. (fun xn =>  bod%comp ) ..))
-    (no associativity, at level 94, id at level 0,
-     x1 closed binder, xn closed binder,
-     format "'Def'  'Constructor'  id  x1  ..  xn  :  'rep'  :=  '/' '[  '   bod ']' " ) :
-consDef_scope.
-
-
-  Delimit Scope ADTParsing_scope with ADTParsing.
-Print BuildADTSig.
-Notation "'ADTRep' r { cons1 , meth1 , .. , methn } " :=
-  (let _ := {| repHint := r |} in
-   (let g := (@BuildADT r
-             _ _
-             _ _
-             (icons cons1%consDef (@inil _ (@consDef r)))
-             (icons meth1%methDefParsing .. (icons methn%methDefParsing (@inil _ (@methDef r))) ..)) in g))
-    (no associativity, at level 96, r at level 0,
-     format "'ADTRep'  r   '/' '[hv  ' {  cons1 ,  '//' meth1 , '//' .. , '//' methn  ']' }") : ADTParsing_scope.
-
-Definition foozbar := option Value.
-
-  Definition CacheSpec : ADT _ :=
+  Definition CacheSpec : ADT CacheSig :=
     (ADTRep (Ensemble (Key * Value)) {
-        Def Constructor "EmptyCache" (t : unit) : rep :=
-          ret (fun _ => False),
-        Def Method "AddKey" (r : rep) (k : Key) (v : Value) : bool :=
-            { r' | (SubEnsembleInsert (k, v) r (fst r')) /\
-                   ((usedKey r k /\ snd r' = false) \/
-                    (~ usedKey r k /\ snd r' = true))},
-        Def Method "UpdateKey" (r : rep) (k : Key) (v : Value -> Value) : bool :=
-              { r' |
-                (Same_set _ (fst r') (EnsembleUpdate k r v))
-                 /\ ((usedKey r k /\ snd r' = true) \/
-                     (~ usedKey r k -> snd r' = false))},
-        Def Method "LookupKey" (r : rep) (k : Key) (v' : Value) : (foozbar) :=
-                v <- {v | ValidLookup r k v};
-        ret (r, v)
-      }%ADTParsing) : ADT _.
+       Def Constructor0 "EmptyCache" : rep :=
+         ret (Empty_set _),
+       Def Method2 "AddKey" (r : rep) (k : Key) (v : Value) : rep * bool :=
+         { r' | (SubEnsembleInsert (k, v) r (fst r')) /\
+                ((usedKey r k /\ snd r' = false) \/
+                 (~ usedKey r k /\ snd r' = true))},
+       Def Method2 "UpdateKey" (r : rep) (k : Key) (v : Value -> Value) : rep * bool :=
+           { r' |
+             (Same_set _ (fst r') (EnsembleUpdate k r v))
+             /\ ((usedKey r k /\ snd r' = true) \/
+                 (~ usedKey r k -> snd r' = false))},
+           Def Method1 "LookupKey" (r : rep) (k : Key) : rep * option Value :=
+             v <- {v | ValidLookup r k v};
+       ret (r, v)
+     }%ADTParsing) : ADT _.
 
-End CacheADT.
+End NotationExample.
