src/QueryStructure/Specification/Representation/TupleADT2.v
@@ -35,16 +35,17 @@ Section TupleADT2.
   Definition InitTuple2 : InitTuple2Dom -> Tuple2 := id.
 
   Definition InitTuple2Def :=
-    Def Constructor Tuple2_Init (inits : InitTuple2Dom) : rep :=
-      InitTuple2 inits.
+    let _ := {| repHint := Tuple2 |} in
+    Def Constructor1 Tuple2_Init (inits : InitTuple2Dom) : rep :=
+      ret (InitTuple2 inits).
 
   (* Getters and Setters for Tuple2s *)
 
   Definition GetTuple2Sig id aType :=
-    Method ("Get" ++ id) : rep x unit -> rep x aType.
+    Method ("Get" ++ id) : rep -> rep * aType.
 
   Definition SetTuple2Sig id aType :=
-    Method ("Set" ++ id) : rep x aType -> rep x unit.
+    Method ("Set" ++ id) : rep * aType -> rep.
 
   Definition Tuple2Sigs'
              {n'}
@@ -69,16 +70,16 @@ Section TupleADT2.
              (attr : Fin.t (NumAttr2 heading)) :
     cMethDef (Rep := @Tuple2 heading) (GetTuple2Sig (Vector.nth (HeadingNames2 heading) attr)
                                                   (Vector.nth (AttrList2 heading) attr)) :=
-    Def Method _ (msg : rep, g : unit)
-    : Vector.nth (AttrList2 heading) attr :=
+    Def Method _ (msg : rep)
+    : rep * (Vector.nth (AttrList2 heading) attr) :=
       (msg, ith2 msg attr).
 
   Definition SetTuple2Def
              (attr : Fin.t (NumAttr2 heading)) :
     cMethDef (Rep := @Tuple2 heading) (SetTuple2Sig (Vector.nth (HeadingNames2 heading) attr)
                                                   (Vector.nth (AttrList2 heading) attr)) :=
-    Def Method _ (msg : rep, val : Vector.nth (AttrList2 heading) attr) : unit :=
-      (replace_Index2 _ msg attr val, tt).
+    Def Method _ (msg : rep) (val : Vector.nth (AttrList2 heading) attr) : rep :=
+      replace_Index2 _ msg attr val.
 
   Definition Tuple2Defs'
            {n'}
@@ -120,14 +121,14 @@ Section TupleADT2.
       BuildADTSig (Vector.cons _ InitTuple2Sig _ (Vector.nil _))
                   Tuple2Sigs.
 
-    Definition Tuple2ADT : cADT Tuple2ADTSig :=
-      BuildcADT (icons InitTuple2Def inil) Tuple2Defs.
+    (*Definition Tuple2ADT : cADT Tuple2ADTSig :=
+      BuildcADT (icons InitTuple2Def inil) Tuple2Defs. *)
 
     (* Support for building messages. *)
 
 
-    Definition ConstructTuple2 subtopics :=
-      CallConstructor Tuple2ADT Tuple2_Init subtopics.
+    (*Definition ConstructTuple2 subtopics :=
+      CallConstructor Tuple2ADT Tuple2_Init subtopics. *)
 
     (* Support for calling message getters. *)
     Lemma BuildGetTuple2MethodID_ibound'
@@ -155,10 +156,10 @@ Section TupleADT2.
                       boundi := BuildGetTuple2MethodID_ibound' _ _ idx |}
       |}.
 
-    Definition CallTuple2GetMethod
+    (*Definition CallTuple2GetMethod
                (r : Tuple2)
                idx
-      := cMethods Tuple2ADT (ibound (indexb (BuildGetTuple2MethodID idx))) r.
+      := cMethods Tuple2ADT (ibound (indexb (BuildGetTuple2MethodID idx))) r. *)
 
     (* Support for calling message setters. *)
     Lemma BuildSetTuple2MethodID_ibound
@@ -186,18 +187,18 @@ Section TupleADT2.
                       boundi := BuildSetTuple2MethodID_ibound _ _ idx |}
       |}.
 
-    Definition CallTuple2SetMethod
+    (*Definition CallTuple2SetMethod
                (r : Tuple2)
                idx
-      := cMethods Tuple2ADT (ibound (indexb (BuildSetTuple2MethodID idx))) r.
+      := cMethods Tuple2ADT (ibound (indexb (BuildSetTuple2MethodID idx))) r. *)
 
 End TupleADT2.
 
-Definition CallDecTuple2GetMethod
+(*Definition CallDecTuple2GetMethod
            {n attrs}
            (r : @DecTuple2 n attrs)
            idx
-  := cMethods (Tuple2ADT _) (ibound (indexb (BuildGetTuple2MethodID _ idx))) r.
+  := cMethods (Tuple2ADT _) (ibound (indexb (BuildGetTuple2MethodID _ idx))) r. *)
 
 (* Notation "t ! R" :=
   (@CallDecTuple2GetMethod _ _ t%Tuple2 (ibound (indexb ((@Build_BoundedIndex _ _ _ R%string _)))) ())
